Update checking artifact (#20)
* include lean updates

* update coq mech

* update content list

checking/lean_v2/data.py
@@ -1,0 +1,83 @@
+#!/usr/bin/env python3
+import subprocess
+import json
+import argparse
+import matplotlib.pyplot as plt
+import numpy as np
+
+parser = argparse.ArgumentParser()
+parser.add_argument("--no-exec", action="store_true")
+parser.add_argument("--log-file", default="data.log")
+parser.add_argument("--fig-file", default="data-{}.pdf")
+args = parser.parse_args()
+
+if args.no_exec:
+    with open(args.log_file) as f:
+        output0 = f.read()
+else:
+    print(r"%running")
+    output0 = subprocess.getoutput("lake lean Lean4/ChkExamples.lean")
+    with open(args.log_file, "w") as f:
+        f.write(output0)
+
+output = output0.replace("(42)", "\"42\"") \
+    .replace("(\"", "[\"") \
+    .replace("})", "}],") \
+    .replace(" :=", "\":") \
+    .replace("{ ", "{ \"") \
+    .replace(", ", ", \"")
+output = "[" + output[:-1] + "]"
+data = []
+for name, time, cnt_ast, cnt_alg in json.loads(output):
+    res = dict(name=name, time=time)
+    res.update(cnt_ast)
+    res.update(cnt_alg)
+    res.pop("world")
+    data.append(res)
+
+config = [
+    ("testcase", lambda x: r"\textsc{" + x["name"] + "}"),
+    ("ast size", lambda x: x["terms"] + x["types"] + x["types"]),
+    ("\\#qual", lambda x: x["types"]),
+    ("time (ms)", lambda x: "%.2f" % x["time"]),
+    ("\\#unif.", lambda x: x["cnt_unify"]),
+    ("\\#infer", lambda x: x["cnt_growth"] + x["cnt_avoid"] + x["cnt_inferqf"]),
+]
+alignstr = "l" + (len(config) - 1) * "r"
+print(r"\begin{tabular}{", alignstr, r"} \toprule", sep="")
+for idx, (col, _) in enumerate(config):
+    print("&\t" * bool(idx), r"\textsc{", col, "}", sep="", end="\t")
+print(r"\\", r"\midrule")
+for res in data:
+    if res["name"].startswith("benchnat"): continue
+    for idx, (_, col) in enumerate(config):
+        print("&\t" * bool(idx), col(res), sep="", end="\t")
+    print(r"\\")
+print(r"\bottomrule \end{tabular}")
+
+datalist = [[], []]
+for i in data:
+    data2 = datalist[1] if i["name"].startswith("benchnat-") else datalist[0]
+    data2.append(i)
+
+for idx, data2 in enumerate(datalist, 1):
+    nterms = np.array([i["terms"] for i in data2])
+    ntypes = np.array([i["types"] for i in data2])
+    sizes = nterms + ntypes
+    times = np.array([i["time"] for i in data2])
+    coeff = np.polyfit(sizes, times, idx)
+    print('%', coeff)
+    model = np.poly1d(coeff)
+    x = np.arange(0, sizes.max() + 50, 50)
+    y = model(x)
+
+    fig, ax = plt.subplots()
+    ax.plot(x, y, c="tab:orange")
+    ax.scatter(sizes, times, marker="x")
+    ax.set_xlim(0, sizes.max())
+    ax.set_xlabel("ast size")
+    ax.set_ylim(0, max(times.max(), y.max()))
+    ax.set_ylabel('time (ms)')
+    fig.set_size_inches(3.2, 4.8)
+    fig.tight_layout()
+    fig.savefig(args.fig_file.format(idx))
