checking/lean_v2/Lean4.lean
@@ -1,0 +1,10 @@
+-- This module serves as the root of the `Lean4` library.
+-- Import modules here that should be built as part of the library.
+import Lean4.LRSound
+import Lean4.ChkTheorems
+-- import Lean4.ChkExamples
+
+namespace Reachability
+
+#print axioms type_safety
+#print axioms embedding.checking_sound
