checking/lean_v2/Lean4/ChkExamples.lean
@@ -1,0 +1,794 @@
+import Lean4.Checking
+
+namespace Reachability.embedding
+
+syntax "⊤": rttype
+syntax "Unit": rttype
+syntax ident: rttype
+syntax "Ref[" rttype "~" rtqual "]": rttype
+syntax "(" (rtid)? "(" rtid ":" rttype "~" rtqual ")" "→" rttype "~" rtqual ")": rttype
+syntax "(∀" (rtid)? "[" rtid "<:" rttype "~" rtqual "]." rttype "~" rtqual ")": rttype
+
+macro_rules
+| `([rttype| ⊤]) => `(fun (_: ℕ) =>
+  ty.TTop)
+| `([rttype| Unit]) => `(fun (_: ℕ) =>
+  ty.TBool)
+| `([rttype| $X:ident]) => `(fun (_: ℕ) =>
+  ty.TVar $X)
+| `([rttype| Ref[$T ~ $q]]) => `(fun (n: ℕ) =>
+  ty.TRef ([rttype| $T] n) [rtqual| $q])
+| `([rttype| ($f($x : $T1 ~ $q1) → $T2 ~ $q2)]) => `(fun (n: ℕ) =>
+  let [rtid| $f] := %n; ty.TFun' n
+    ([%n ↦ #0] [rttype| $T1] (n+1))
+    ([%n ↦ #0] [rtqual| $q1])
+    (let [rtid| $x] := %(n+1); [rttype| $T2] (n+2))
+    (let [rtid| $x] := %(n+1); [rtqual| $q2]))
+| `([rttype| (∀$f[$x <: $T1 ~ $q1]. $T2 ~ $q2)]) => `(fun (n: ℕ) =>
+  let [rtid| $f] := %n; ty.TAll' n
+    ([%n ↦ #0] [rttype| $T1] (n+1))
+    ([%n ↦ #0] [rtqual| $q1])
+    (let [rtid| $x] := %(n+1); [rttype| $T2] (n+2))
+    (let [rtid| $x] := %(n+1); [rtqual| $q2]))
+| `([rttype| (($x : $T1 ~ $q1) → $T2 ~ $q2)]) => `([rttype| (_($x : $T1 ~ $q1) → $T2 ~ $q2)])
+| `([rttype| (∀[$X <: $T1 ~ $q1]. $T2 ~ $q2)]) => `([rttype| (∀_[$X <: $T1 ~ $q1]. $T2 ~ $q2)])
+
+syntax "unit": rtterm
+syntax:max ident: rtterm
+syntax "ref" rtterm: rtterm
+syntax "!" rtterm: rtterm
+syntax rtterm ":=" rtterm: rtterm
+syntax rtterm rtterm:max : rtterm
+syntax rtterm "[" rttype "~" rtqual "]" : rtterm
+syntax "lam" (rtid)? "(" rtid ") ." rtterm : rtterm
+syntax "lam" (rtid)? "(" rtid ":" rttype "~" rtqual ") ." rtterm : rtterm
+syntax "lam" (rtid)? "[" rtid "<:" rttype "~" rtqual "] ." rtterm : rtterm
+syntax "(" rtterm ":" rttype "~" rtqual ")": rtterm
+syntax "let" rtid "=" rtterm "in" rtterm: rtterm
+syntax "let" "(" rtid ":" rttype "~" rtqual ")" "=" rtterm "in" rtterm: rtterm
+
+macro_rules
+| `([rtterm| unit]) => `(fun (_: ℕ) =>
+  tm.tfalse)
+| `([rtterm| $x:ident]) => `(fun (_: ℕ) =>
+  tm.tvar! $x)
+| `([rtterm| ref $t]) => `(fun (n: ℕ) =>
+  tm.tref ([rtterm| $t] n))
+| `([rtterm| ! $t]) => `(fun (n: ℕ) =>
+  tm.tget ([rtterm| $t] n))
+| `([rtterm| $t1 := $t2]) => `(fun (n: ℕ) =>
+  tm.tput ([rtterm| $t1] n) ([rtterm| $t2] n))
+| `([rtterm| $t1 $t2]) => `(fun (n: ℕ) =>
+  tm.tapp ([rtterm| $t1] n) ([rtterm| $t2] n))
+| `([rtterm| $t1 [ $T ~ $q ]]) => `(fun (n: ℕ) =>
+  tm.ttapp ([rtterm| $t1] n) ([rttype| $T] n) [rtqual| $q])
+| `([rtterm| lam $f($x) . $body]) => `(fun (n: ℕ) =>
+  let [rtid|$f] := %n; let [rtid|$x] := %(n+1);
+  tm.tabs ([rtterm| $body] (n+2)))
+| `([rtterm| lam $f($x : $T ~ $q) . $body]) => `(fun (n: ℕ) =>
+  let [rtid| $f] := %n; tm.tabsa
+    ([%n ↦ #0] [rttype| $T] (n+1))
+    ([%n ↦ #0] [rtqual| $q])
+    (let [rtid| $x] := %(n+1); [rtterm| $body] (n+2)))
+| `([rtterm| lam $f[$X <: $T ~ $q] . $body]) => `(fun (n: ℕ) =>
+  let [rtid| $f] := %n; tm.ttabs
+    ([%n ↦ #0] [rttype| $T] (n+1))
+    ([%n ↦ #0] [rtqual| $q])
+    (let [rtid| $X] := %(n+1); [rtterm| $body] (n+2)))
+| `([rtterm| ($t : $T ~ $q)]) => `(fun (n: ℕ) =>
+  tm.tanno ([rtterm| $t] n) ([rttype| $T] n) [rtqual| $q])
+| `([rtterm| let $x = $t1 in $t2]) => `([rtterm| (lam _($x) . $t2) $t1])
+| `([rtterm| let ($x : $T ~ $q) = $t1 in $t2]) => `([rtterm| let $x = ($t1 : $T ~ $q) in $t2])
+| `([rtterm| lam ($x) . $body]) => `([rtterm| lam _($x) . $body])
+| `([rtterm| lam ($x : $T ~ $q) . $body]) => `([rtterm| lam _($x : $T ~ $q) . $body])
+| `([rtterm| lam [$X <: $T ~ $q] . $body]) => `([rtterm| lam _[$X <: $T ~ $q] . $body])
+
+
+section Church_Bool
+
+def ty.CBool := [rttype|
+  (∀[T <: ⊤ ~{✦, #0}]. ((x: T ~{✦, #0}) → ((y: T ~{✦, #0}) → T ~{x, y}) ~{x}) ~∅)
+]
+
+def ctrue := [rtterm|
+  lam [T <: ⊤ ~{✦, #0}] . lam (x: T ~{✦, #0}) . lam (_: T ~{✦, #0}) . x
+]
+
+def cfalse := [rtterm|
+  lam [T <: ⊤ ~{✦, #0}] . lam (_: T ~{✦, #0}) . lam (x: T ~{✦, #0}) . x
+]
+
+syntax "Bool": rttype
+macro_rules
+| `([rttype| Bool]) => `(ty.CBool)
+
+def ccond := [rtterm|
+  lam [T <: ⊤ ~{✦, #0}] . lam (b: Bool ~{✦, #0}) . b [T ~{T}]
+]
+
+syntax "true": rtterm
+syntax "false": rtterm
+syntax "cond": rtterm
+macro_rules
+| `([rtterm| true]) => `([rtterm| (⟪ctrue⟫: Bool ~∅)])
+| `([rtterm| false]) => `([rtterm| (⟪cfalse⟫: Bool ~∅)])
+| `([rtterm| cond]) => `(ccond)
+
+def andb := [rtterm|
+  lam (x: Bool ~∅) . lam (y: Bool ~∅) . x [Bool ~∅] y true
+]
+def orb := [rtterm|
+  lam (x: Bool ~∅) . lam (y: Bool ~∅) . x [Bool ~∅] true y
+]
+def negb := [rtterm|
+  lam (x: Bool ~∅) . x [Bool ~∅] false true
+]
+
+def cbool_example := [rtterm|
+  (let x = ref true in x: Ref[Bool ~∅] ~{✦})
+]
+#eval check_program cbool_example
+
+end Church_Bool
+
+
+section Church_Nat
+
+-- (A → A) → A → A
+def ty.TNat := [rttype|
+  (∀[A <: ⊤ ~{✦, #0}].
+    ((_: ((_: A ~{A}) → A ~{A}) ~ {#0, ✦}) →
+    ((_: A ~{A}) → A ~{A}) ~{#0, #1}) ~{#0, #1})
+]
+
+syntax "Nat": rttype
+macro_rules
+| `([rttype| Nat]) => `(ty.TNat)
+
+-- Λ[X]. λf.λx. x
+def zero := [rtterm|
+  lam [X <: ⊤ ~{#0, ✦}] .
+    lam (_ : ((_: X ~{X}) → X ~{X}) ~{#0, ✦}) .
+      lam (x : X ~{X}) .
+        x
+]
+#eval check_program zero
+
+def one := [rtterm|
+  lam [X <: ⊤ ~{#0, ✦}] .
+    lam (f : ((_: X ~{X}) → X ~{X}) ~{#0, ✦}) .
+      lam (x : X ~{X}) .
+        f x
+]
+#eval check_program one
+
+-- λn. λf. λx. f (n f x)
+def succ := [rtterm|
+  lam (n : Nat ~{✦, #0}) .
+    lam [X <: ⊤ ~{#0, ✦}] .
+      lam (f : ((_: X ~{X}) → X ~{X}) ~{#0, ✦}) .
+        lam (x : X ~{X}) .
+          f (n [X ~{X}] f x)
+]
+#eval check_program succ
+
+def nadd := [rtterm|
+  lam (m: Nat ~∅) . lam (n: Nat ~∅) .
+    m [Nat ~∅] ⟪succ⟫ n
+]
+
+def nmul := [rtterm|
+  lam (m: Nat ~∅) . lam (n: Nat ~∅) . lam [X <: ⊤ ~{#0, ✦}] .
+    lam (f : ((_: X ~{X}) → X ~{X}) ~{#0, ✦}) .
+    n [X ~{X}] (m [X ~{X}] f)
+]
+
+def nrepeat := [rtterm|
+  lam (n: Nat ~∅) . lam (f: ((_: Nat ~∅) → Unit ~∅) ~{✦, #0}) .
+    n [Nat ~∅] (lam (i) . let _ = f i in ⟪succ⟫ i) ⟪zero⟫
+]
+#eval check_program nrepeat
+
+def translate_num (n: ℕ) :=
+  if n > 2 then
+    [rtterm| let succ = ⟪succ⟫ in ⟪go [rtterm| succ] n⟫]
+  else go succ n
+where go (succ: ℕ → tm): ℕ → ℕ → tm
+  | 0 => zero
+  | 1 => one
+  | n + 1 => [rtterm| ⟪succ⟫ ⟪translate_num.go succ n⟫]
+
+syntax:max num: rtterm
+syntax:60 rtterm:60 "+" rtterm:61: rtterm
+syntax:70 rtterm:70 "*" rtterm:71: rtterm
+syntax "for" rtid "<" rtterm "in" rtterm: rtterm
+macro_rules
+| `([rtterm| $n:num]) => `([rtterm| (⟪translate_num $n⟫ : Nat ~∅)])
+| `([rtterm| $m + $n]) => `([rtterm| ⟪nadd⟫ $m $n])
+| `([rtterm| $m * $n]) => `([rtterm| (⟪nmul⟫ $m $n : Nat ~∅)])
+| `([rtterm| for $x < $n in $body]) => `([rtterm| ⟪nrepeat⟫ $n (lam ($x) . $body)])
+
+def cnat_example := [rtterm|
+  let x = ref (1 + 1 * 2) in
+  let (_: Ref[Nat ~∅] ~{x}) = x in
+  let _ =
+    for i < 10 in
+      x := (!x) + i in
+  ! x
+]
+#eval check_program cnat_example
+
+-- ∀a. ((a → a) → a → a) → ((a → a) → a → a) → (a → a) → a → a
+-- λm. λn. λf. λx. m (n f) x
+def pow := [rtterm| --m^n
+  lam (m : Nat ~∅) . lam (n : Nat ~∅) .
+    -- (lam [X <: ⊤ ~{#0, ✦}] . n [((_: X ~{X}) → X ~{X}) ~{X}] (m [X ~{X}]): Nat ~∅)
+    n [Nat ~∅] (lam (x) . m * x) 1
+]
+
+#eval check_program pow
+
+def pow_example := [rtterm|
+  let n0 = 0 in
+  let n1 = 1 in
+  let succ = ⟪succ⟫ in
+  let n2 = succ n1 in
+  let n3 = succ n2 in
+  let pow = ⟪pow⟫ in
+  let n9 = pow n3 n2 in
+  let (_: Nat ~∅) = n0 in
+  let (_: Nat ~∅) = n1 in
+  let (_: Nat ~∅) = n2 in
+  let (_: Nat ~∅) = n3 in
+  let (_: Nat ~∅) = n9 in
+  n9
+]
+
+#eval check_program pow_example
+
+end Church_Nat
+
+
+section escapingpairs
+
+def ty.TPair (X : ℕ → ty) (qx : ql) (Y : ℕ → ty) (qy : ql) := [rttype|
+  (∀[R <: ⊤~{#0,✦}]. (
+    (_: ((_: ⟪X⟫ ~ qx) → ((_: ⟪Y⟫ ~ qy) → R ~{R}) ~{#0, #1}) ~{✦, #0}) →
+    R ~{R}
+  )~{#0,#1})
+]
+
+syntax "(" rttype "~" rtqual "⊗" rttype "~" rtqual ")": rttype
+macro_rules
+| `([rttype| ($X ~ $qx ⊗ $Y ~ $qy)]) => `(fun (n: ℕ) =>
+  ty.TPair [rttype| $X] [rtqual| $qx] [rttype| $Y] [rtqual| $qy] n)
+
+def mkpair := [rtterm|
+  lam [A <: ⊤ ~{#0, ✦}] . lam [B <: ⊤ ~{#0, ✦}] .
+  lam (a: A ~{A}) . lam (b: B ~{B}) .
+  lam [C <: ⊤ ~{#0, ✦}] . lam (f: ((_: A ~{A}) → ((_: B ~{B}) → C ~{C}) ~{#0, #1}) ~{✦, #0}) .
+  f a b
+]
+
+#eval check_program mkpair
+
+def tfst := [rtterm|
+  lam (x) . lam (_) . x
+]
+
+def tsnd := [rtterm|
+  lam (_) . lam (y) . y
+]
+
+def tfst' := [rtterm|
+  lam [X <: ⊤ ~{#0, ✦}] . lam [Y <: ⊤ ~{#0, ✦}] .
+  lam (p: (X ~{X} ⊗ Y ~{Y}) ~{#0, ✦}) .
+    p [X ~{X}] ⟪tfst⟫
+]
+
+#eval check_program tfst'
+
+def tsnd' := [rtterm|
+  lam [X <: ⊤ ~{#0, ✦}] . lam [Y <: ⊤ ~{#0, ✦}] .
+  lam (p : (X ~{X} ⊗ Y ~{Y}) ~{#0, ✦}) .
+    p [Y ~{Y}] ⟪tsnd⟫
+]
+
+#eval check_program tsnd'
+
+def transparent_pair := [rtterm|
+  let mkpair = ⟪mkpair⟫ in
+  let x = ref true in
+  let y = ref false in
+  let p = mkpair [Ref[Bool~∅] ~{x}] [Ref[Bool~∅] ~{y}] x y in
+  let (_ : Ref[Bool~∅] ~{x}) = p [Ref[Bool~∅] ~{x}] ⟪tfst⟫ in
+  let (_ : Ref[Bool~∅] ~{y}) = p [Ref[Bool~∅] ~{y}] ⟪tsnd⟫ in
+  let (_ : Ref[Bool~∅] ~{x}) = ⟪tfst'⟫ [Ref[Bool~∅] ~{x}] [Ref[Bool~∅] ~{y}] p in
+  let (_ : Ref[Bool~∅] ~{y}) = ⟪tsnd'⟫ [Ref[Bool~∅] ~{x}] [Ref[Bool~∅] ~{y}] p in
+  true
+]
+
+#eval check_program transparent_pair
+#eval bench_program "pair-trans" transparent_pair
+
+def opaque_pair := [rtterm|
+  let p = (
+    let mkpair = ⟪mkpair⟫ in
+    let x = ref true in
+    let y = ref false in
+    let p = mkpair [Ref[Bool~∅] ~{x}] [Ref[Bool~∅] ~{y}] x y in
+    p) in
+  let (_ : Ref[Bool~∅] ~{p}) = p [Ref[Bool~∅] ~{p}] ⟪tfst⟫ in
+  let (_ : Ref[Bool~∅] ~{p}) = p [Ref[Bool~∅] ~{p}] ⟪tsnd⟫ in
+  let (_ : Ref[Bool~∅] ~{p}) = ⟪tfst'⟫ [Ref[Bool~∅] ~{p}] [Ref[Bool~∅] ~{p}] p in
+  let (_ : Ref[Bool~∅] ~{p}) = ⟪tsnd'⟫ [Ref[Bool~∅] ~{p}] [Ref[Bool~∅] ~{p}] p in
+  true
+]
+
+#eval check_program opaque_pair
+#eval bench_program "pair-opaque" opaque_pair
+
+end escapingpairs
+
+
+section safepar
+
+def par := [rtterm|
+  lam (f : ((_: Unit~∅) → Unit~∅) ~{✦}) .
+    lam (g : ((_: Unit~∅) → Unit~∅) ~{✦}) .
+      (unit: Unit~{f, g}) -- simulate using incr, decr
+]
+#eval check_program par
+
+def safepar_var := [rtterm|
+  let par = ⟪par⟫ in
+  let a = ref 0 in
+  let b = ref 0 in
+  let _ = a in
+  par (lam (_) . a := (!a) + 1) (lam (_) . b := (!b) + 1)
+]
+#eval check_program safepar_var
+#eval bench_program "par-var1" safepar_var
+
+def unsafepar_var := [rtterm|
+  let par = ⟪par⟫ in
+  let a = ref 0 in
+  let _ = ref 0 in
+  let c = a in
+  par (lam (_) . a := (!a) + 1) (lam (_) . c := (!c) + 1)
+]
+#guard_msgs (drop error) in #eval check_program unsafepar_var
+#eval bench_program "par-var2" unsafepar_var
+
+def safepar_fun := [rtterm|
+  let par = ⟪par⟫ in
+  let inc = lam (x: Ref[Nat ~∅] ~{✦}) . x := (!x) + 1 in
+  let a = ref 0 in
+  let b = ref 0 in
+  par (lam (_) . inc a) (lam (_) . inc b)
+]
+#eval check_program safepar_fun
+#eval bench_program "par-fun1" safepar_fun
+
+def unsafepar_fun := [rtterm|
+  let par = ⟪par⟫ in
+  let inc = (let d = ref 0 in
+    lam (_: Ref[Nat ~∅] ~{✦}) . d := (!d) + 1) in
+  let a = ref 0 in
+  let b = ref 0 in
+  par (lam (_) . inc a) (lam (_) . inc b)
+]
+#guard_msgs (drop error) in #eval check_program unsafepar_fun
+#eval bench_program "par-fun2" unsafepar_fun
+
+def safepar_ref := [rtterm|
+  let par = ⟪par⟫ in
+  let a = ref 0 in
+  let b = ref 0 in
+  let a1 = ref a in
+  let b1 = ref b in
+  par (lam (_) . (!a1) := (!!a1) + 1) (lam (_) . (!b1) := (!!b1) + 1)
+]
+#eval check_program safepar_ref
+#eval bench_program "par-ref1" safepar_ref
+
+def unsafepar_ref := [rtterm|
+  let par = ⟪par⟫ in
+  let a = ref 0 in
+  let _ = ref 0 in
+  let a1 = ref a in
+  let b1 = ref a in
+  par (lam (_) . (!a1) := (!!a1) + 1) (lam (_) . (!b1) := (!!b1) + 1)
+]
+#guard_msgs (drop error) in #eval check_program unsafepar_ref
+#eval bench_program "par-ref2" unsafepar_ref
+
+def counter := [rtterm|
+  lam (n : Nat ~∅) .
+    let c = ref n in
+    ⟪mkpair⟫ [((_: Unit~∅) → Unit~∅) ~{c}] [((_: Unit ~∅) → Unit~∅) ~{c}]
+      (lam (_) . c := (!c) + 1) (lam (_) . c := (!c) + 1)
+]
+
+#eval check_program counter
+
+def sequential_counter_example := [rtterm|
+  let ctr = ⟪counter⟫ 0 in
+  let incr = ⟪tfst'⟫ [((_: Unit~∅) → Unit~∅) ~{ctr}] [((_: Unit~∅) → Unit~∅) ~{ctr}] ctr in
+  let decr = ⟪tsnd'⟫ [((_: Unit~∅) → Unit~∅) ~{ctr}] [((_: Unit~∅) → Unit~∅) ~{ctr}] ctr in
+  let (_: ((_: Unit~∅) → Unit~∅) ~{ctr}) = incr in
+  let (_: ((_: Unit~∅) → Unit~∅) ~{ctr}) = decr in
+  let (_: Unit~∅) = incr unit in  -- should apply on unit
+  let (_: Unit~∅) = decr unit in
+  ctr
+]
+
+#eval check_program sequential_counter_example
+#eval bench_program "seq-ctr" sequential_counter_example
+-- #eval bench_program "par" par
+
+def affirmative_par_example := [rtterm|
+  let counter = ⟪counter⟫ in
+  let ctr1 = counter 0 in
+  let ctr2 = counter 0 in
+  let incr1 = ⟪tfst'⟫ [((_: Unit~∅) → Unit~∅) ~{ctr1}] [((_: Unit~∅) → Unit~∅) ~{ctr1}] ctr1 in
+  let decr2 = ⟪tsnd'⟫ [((_: Unit~∅) → Unit~∅) ~{ctr2}] [((_: Unit~∅) → Unit~∅) ~{ctr2}] ctr2 in
+  -- let (_: ((_: ((_: Unit~∅) → Unit~∅)~{✦}) → Unit~∅) ~{incr}) = ⟪par⟫ incr in
+  let _ = ⟪par⟫ incr1 decr2 in -- error here
+  false
+]
+
+#eval check_program affirmative_par_example
+#eval bench_program "par-ctr1" affirmative_par_example
+
+-- negative example, expect failure
+def negative_par_example := [rtterm|
+  let ctr = ⟪counter⟫ 0 in
+  let incr = ⟪tfst'⟫ [((_: Unit~∅) → Unit~∅) ~{ctr}] [((_: Unit~∅) → Unit~∅) ~{ctr}] ctr in
+  let decr = ⟪tsnd'⟫ [((_: Unit~∅) → Unit~∅) ~{ctr}] [((_: Unit~∅) → Unit~∅) ~{ctr}] ctr in
+  -- let (_: ((_: ((_: Unit~∅) → Unit~∅)~{✦}) → Unit~∅) ~{incr}) = ⟪par⟫ incr in
+  let _ = ⟪par⟫ incr decr in -- error here
+  false
+]
+
+#guard_msgs (drop error) in #eval check_program negative_par_example
+#eval bench_program "par-ctr2" negative_par_example
+
+def parshared := [rtterm|
+  lam (a : ⊤~{✦, #0}) .
+  lam (f : ((_: Unit~∅) → Unit~∅) ~{✦,a}) .
+    lam (g : ((_: Unit~∅) → Unit~∅) ~{✦,a}) .
+      (unit: Unit~{f, g}) -- simulate using incr, decr
+]
+#eval check_program parshared
+
+def parshared_example1 := [rtterm|
+  let par = ⟪parshared⟫ in
+  let a = ref 0 in
+  let b = ref 0 in
+  let c = ref 1 in
+  par c (lam (_) . a := (!a) + (!c)) (lam (_) . b := (!b) + (!c))
+]
+#eval check_program parshared_example1
+#eval bench_program "par-shr1" parshared_example1
+
+def parshared_example2 := [rtterm|
+  let par = ⟪parshared⟫ in
+  let a = ref 0 in
+  let b = ref 0 in
+  let c = ref 1 in
+  par c (lam (_) . a := (!a) + (!c)) (lam (_) . b := (!b) + (!a))
+]
+#guard_msgs (drop error) in #eval check_program parshared_example2
+#eval bench_program "par-shr2" parshared_example2
+
+end safepar
+
+section effectcapability
+
+def try_type (CanThrow: id) := [rttype|
+  (∀[A <: ⊤ ~{#0, ✦}]. ((_: ((_: CanThrow ~{✦}) → A ~{A}) ~{#0, ✦}) → A ~{A}) ~{A})
+]
+
+def throw_type (CanThrow: id) := [rttype|
+  (∀[A <: ⊤ ~{#0, ✦}]. ((_: CanThrow ~{#0, ✦}) → A ~{A}) ~{A})
+]
+
+def try1_safe := [rtterm|
+  lam [CanThrow <: ⊤ ~{#0, ✦}] .
+  lam (try_: ⟪try_type CanThrow⟫ ~{✦}) .
+  lam (throw_: ⟪throw_type CanThrow⟫ ~∅) .
+  try_ [Nat ~∅] (lam (c) . throw_ [Nat ~∅] c)
+]
+
+#eval check_program try1_safe
+#eval bench_program "try-safe" try1_safe
+
+def try2_escape := [rtterm|
+  lam [CanThrow <: ⊤ ~{#0, ✦}] .
+  lam (try_: ⟪try_type CanThrow⟫ ~{✦}) .
+  lam (throw_: ⟪throw_type CanThrow⟫ ~∅) .
+  let c = try_ [CanThrow ~{✦}] (lam (c) . c) in
+  throw_ [Bool ~∅] c
+]
+
+#guard_msgs (drop error) in #eval check_program try2_escape
+#eval bench_program "try-esc" try2_escape
+
+def mytry_type (CanThrow: id) := [rttype|
+  ((_: ((_: CanThrow ~{✦, #0}) → Nat ~∅) ~{✦, #0}) → Nat ~∅)
+]
+
+def try3_escf := [rtterm|
+  lam [CanThrow <: ⊤ ~{#0, ✦}] .
+  lam (try_: ⟪try_type CanThrow⟫ ~{✦}) .
+  lam (throw_: ⟪throw_type CanThrow⟫ ~∅) .
+  let mytry = try_ [⟪mytry_type CanThrow⟫ ~{✦}] (lam (c) . lam (f) . f c) in
+  mytry (lam (c) . throw_ [Nat ~∅] c)
+]
+
+#guard_msgs (drop error) in #eval check_program try3_escf
+#eval bench_program "try-fun" try3_escf
+
+def try4_nocap := [rtterm|
+  lam [CanThrow <: ⊤ ~{#0, ✦}] .
+  lam (try_: ⟪try_type CanThrow⟫ ~{✦}) .
+  lam (throw_: ⟪throw_type CanThrow⟫ ~∅) .
+  let nocap = lam [A <: ⊤ ~{#0, ✦}] . lam (cap: CanThrow ~{✦, #0}) . lam (body: ((_: Unit ~∅) → A ~{A}) ~{✦}) .
+    let _ = cap in
+    body unit in
+  try_ [Nat ~∅] (lam (c) . nocap [Nat ~∅] c (lam (_) . throw_ [Nat ~∅] c))
+]
+
+#guard_msgs (drop error) in #eval check_program try4_nocap
+#eval bench_program "try-nocap" try4_nocap
+
+end effectcapability
+
+
+section lists
+
+def nil := [rtterm|
+  lam [A <: ⊤ ~{#0, ✦}] .
+    -- R can depend or not depend on A
+    lam [R <: ⊤ ~{#0, ✦}] .
+      lam (_: ((_: A ~{A}) → ((_: R ~{R}) → R ~{R}) ~{#0}) ~{✦, #0}) .
+        lam (n : R ~{R}) . n
+]
+
+#eval check_program nil
+
+-- NOTE: The inner part is R^R -> R^R instead of (x:R^R) -> x^x
+-- ∀R. (A → R → R) → R → R
+def ty.TList (A : ℕ → ty) (aq : ql) := [rttype|
+  (∀[R <: ⊤ ~{#0, ✦}]. (
+    (_: ((_: ⟪A⟫ ~aq) → ((_: R ~{R}) → R ~{R}) ~{#0, #1}) ~{#0, ✦}) →
+    ((_: R ~{R}) → R ~{R}) ~{#0, #1}
+  ) ~{#0, #1})
+]
+
+def ty.UList (A : ℕ → ty) := [rttype|
+  (∀l[R <: ⊤ ~{#0, ✦}]. (
+    (_: ((_: ⟪A⟫ ~{l}) → ((_: R ~{R}) → R ~{R}) ~{#0, #1}) ~{#0, ✦}) →
+    ((_: R ~{R}) → R ~{R}) ~{#0, #1}
+  ) ~{#0, #1})
+]
+
+syntax "List[" rttype "~" rtqual "]": rttype
+syntax "UList[" rttype "]": rttype
+macro_rules
+| `([rttype| List[$T ~ $q]]) => `(fun (n: ℕ) =>
+  ty.TList [rttype| $T] [rtqual| $q] n)
+| `([rttype| UList[$T]]) => `(fun (n: ℕ) =>
+  ty.UList [rttype| $T] n)
+
+def cons := [rtterm|
+  lam [A <: ⊤ ~{#0, ✦}] .
+    lam (hd : A ~{A}) .
+      lam (tl : List[A ~{A}] ~{A}) .
+        lam [R <: ⊤ ~{#0, ✦}] .
+          lam (c : ((_: A ~{A}) → ((_: R ~{R}) → R ~{R}) ~{#0,#1}) ~{#0,✦}) .
+            lam (n : R ~{R}) . c hd (tl [R ~{R}] c n)
+]
+
+#eval check_program cons
+
+def sum := [rtterm|
+  lam (lst: UList[Ref[Nat~∅]] ~{✦, #0}) .
+    lst [Nat ~∅] (lam (r) . lam (a) . a + (!r)) 0
+]
+#eval check_program sum
+
+def cons_example := [rtterm|
+  let cons = ⟪cons⟫ in
+  let sum = ⟪sum⟫ in
+  let l = (
+    let x = ref 0 in
+    let y = ref 1 in
+    let z = ref 2 in
+    let l0 = ⟪nil⟫ [Ref[Nat~∅] ~∅] in
+    let _ = sum l0 in
+    let l1 = cons [Ref[Nat~∅] ~{x}] x l0 in
+    let _ = sum l1 in
+    let l2 = cons [Ref[Nat~∅] ~{x,y}] y l1 in
+    let _ = sum l2 in
+    let l3 = cons [Ref[Nat~∅] ~{x,y,z}] z l2 in
+    let _ = sum l3 in
+    l3) in
+  let (_: List[Ref[Nat~∅] ~{l}] ~{l}) = l in
+  sum l
+]
+
+#eval check_program cons_example
+#eval bench_program "list-sum" cons_example
+
+-- isnil = λX. λl:List X. l [Bool] (λhd:X. λtl:Bool. false) true
+def isnil := [rtterm|
+  lam [X <: ⊤ ~{#0, ✦}] .
+    lam (l: List[X ~{X}] ~{X}) .
+      l [Bool ~∅] (lam (_) . lam (_) . false) true
+]
+
+#eval check_program isnil
+
+/-
+  map : (X → Y ) → List X → List Y
+  Λa. Λb. λ(f : a → b). λ(xs : ∀r. (a → r → r) → r → r).
+    xs (∀r. (b → r → r) → r → r)
+      (λ(x : a) (acc : ∀r. (b → r → r) → r → r).cons b (f x) acc) (nil b)
+-/
+
+def map := [rtterm|
+  lam [X <: ⊤ ~{#0, ✦}] . lam [Y <: ⊤ ~{#0, ✦}] .
+    lam (f: ((_: X ~{X}) → Y ~{Y}) ~{#0,✦}) .
+      lam (xs: List[X ~{X}] ~{#0,✦}) .
+        -- construction part, List[Y] should alias f
+        xs [List[Y ~{Y}] ~{Y}]
+          (lam (x) . lam (acc) . ⟪cons⟫ [Y ~{Y}] (f x) acc)
+          (⟪nil⟫ [Y ~{Y}])
+]
+
+#eval check_program map
+
+def list := [rtterm|
+  let nil = ⟪nil⟫ in
+  let cons = ⟪cons⟫ in
+  let map = ⟪map⟫ in
+  let isnil = ⟪isnil⟫ in
+  let x = ref true in
+  let y = ref false in
+  let sl = cons [Ref[Bool~∅] ~{x}] x (nil [Ref[Bool~∅] ~{x}]) in
+  let (_: List[Ref[Bool~∅] ~{x}] ~{x}) = sl in
+  let (_: List[Ref[Bool~∅] ~{y}] ~{y}) =
+    map [Ref[Bool~∅] ~{x}] [Ref[Bool~∅] ~{y}] (lam (_) . y) sl in
+  let (_: Bool~∅) = isnil [Ref[Bool~∅] ~{x, y}] sl in
+  sl
+]
+
+#eval check_program list
+#eval bench_program "list-map" list
+
+end lists
+
+
+section seplists
+
+def mnil := [rtterm|
+  lam [A <: ⊤ ~{#0, ✦}] .
+    -- R can dependent or not dependent on A
+    lam [R <: ⊤ ~{✦}] .
+      lam (_ : ((_: A ~{✦}) → ((_: R ~{R}) → R ~{R}) ~{#0,#1}) ~{✦}) .
+        lam (n: R ~{R}) . n
+]
+
+-- NOTE: The inner part is R^R -> R^R instead of (x:R^R) -> x^x
+-- ∀R. (A → R → R) → R → R
+def ty.TList2 (A : ℕ → ty) := [rttype|
+  (∀ [R <: ⊤ ~{✦}]. (
+    (_: ((_: ⟪A⟫ ~{✦}) → ((_: R ~{R}) → R ~{R}) ~ {#0,#1}) ~{✦}) →
+    ((_: R ~{R}) → R ~{R}) ~{#0, #1}
+  ) ~{#0, #1})
+]
+
+syntax "MList[" rttype "]": rttype
+macro_rules
+| `([rttype| MList[$T]]) => `(fun (n: ℕ) =>
+  ty.TList2 [rttype| $T] n)
+
+def mcons := [rtterm|
+  lam [A <: ⊤ ~{#0, ✦}] .
+    lam (hd: A ~{✦}) . lam (tl: MList[A] ~{✦}) .
+      (lam [R <: ⊤ ~{✦}] .
+        lam (c : ((_: A ~{✦}) → ((_: R ~{R}) → R ~{R}) ~{#0,#1}) ~{✦}) .
+          lam (n: R ~{R}) . c hd (tl [R ~{R}] c n)
+      : MList[A] ~{hd,tl})  -- eager coercion to avoid upcasting adding extra variables
+]
+
+def miter := [rtterm|
+  lam [X <: ⊤ ~{#0, ✦}] .
+    lam (f : ((_: X ~{✦}) → Unit ~∅) ~∅) .
+      lam (xs : MList[X] ~{#0,✦}) .
+        -- construction part, List[Y] should alias f
+        xs [Unit ~∅]
+          (lam (x) . lam (_) . f x)
+          unit
+]
+
+#eval check_program miter
+
+def test_list2 := [rtterm|
+  let mcons = ⟪mcons⟫ in
+  let l0 = ⟪mnil⟫ [Ref[Bool~∅] ~{✦}] in
+  let (_: MList[Ref[Bool~∅]] ~∅) = l0  in
+  let x = ref true in
+  let y = ref false in
+  let l1 = mcons [Ref[Bool~∅] ~{✦}] x l0 in
+  let (_ : MList[Ref[Bool~∅]] ~{l1}) = l1 in
+  let l2 = mcons [Ref[Bool~∅] ~{✦}] y l1 in
+  let (_ : MList[Ref[Bool~∅]] ~{l2}) = l2 in
+  let _ = ⟪miter⟫ [Ref[Bool~∅] ~{✦}] (lam (x) . x := !x) l2 in
+  true
+]
+
+#eval check_program test_list2
+#eval bench_program "mlist-sep" test_list2
+
+def test_list2_fail := [rtterm|
+  let mcons = ⟪mcons⟫ in
+  let l0 = ⟪mnil⟫ [Ref[Bool~∅] ~{✦}] in
+  let (_: MList[Ref[Bool~∅]] ~∅) = l0  in
+  let x = ref true in
+  let y = ref false in
+  let l1 = mcons [Ref[Bool~∅] ~{✦}] x l0 in
+  let (_ : MList[Ref[Bool~∅]] ~{l1}) = l1 in
+  let l2 = mcons [Ref[Bool~∅] ~{✦}] y l1 in
+  let _ = mcons [Ref[Bool~∅] ~{✦}] x l2 in
+  true
+]
+
+#guard_msgs (drop error) in #eval check_program test_list2_fail
+#eval bench_program "mlist-shr" test_list2_fail
+
+end seplists
+
+
+section benchnat
+
+def create_bench (n: ℕ) (t: ℕ → tm) :=
+  if n > 5 then
+    [rtterm| let i = ⟪t⟫ + 10 in ⟪create_bench (n - 10) [rtterm| i]⟫]
+  else
+    [rtterm| ⟪t⟫ + ⟪translate_num n⟫]
+
+def benchnat i :=
+  bench_program s!"benchnat-{i}"
+    -- (translate_num i)
+    (create_bench i zero)
+    -- (translate_num.go succ i)
+
+#eval benchnat 10
+#eval benchnat 20
+#eval benchnat 30
+#eval benchnat 40
+#eval benchnat 50
+#eval benchnat 60
+#eval benchnat 70
+#eval benchnat 80
+#eval benchnat 90
+#eval benchnat 100
+#eval benchnat 110
+#eval benchnat 120
+#eval benchnat 130
+#eval benchnat 140
+#eval benchnat 150
+#eval benchnat 160
+#eval benchnat 170
+#eval benchnat 180
+#eval benchnat 190
+#eval benchnat 200
+#eval benchnat 210
+#eval benchnat 220
+#eval benchnat 230
+#eval benchnat 240
+
+end benchnat
