checking/lean_v2/Lean4/LangDefs.lean
@@ -1,0 +1,332 @@
+import Mathlib.Data.Finset.Basic
+import Mathlib.Data.Finset.Image
+import Lean4.Attrs
+
+notation:max "‖" L "‖" => List.length L
+notation:max "?[" b "]" s:66 => if b then s else ∅
+
+namespace Reachability
+
+-- identifier
+
+inductive id: Type
+| fresh
+| bv (n: Nat)
+| fv (n: Nat)
+deriving DecidableEq
+
+class Subst (α β: Type) where
+  subst: id → β → α → α
+
+export Subst (subst)
+
+notation:max "[" x "↦" xs "]" q:66 =>  Subst.subst x xs q
+
+notation "✦" => id.fresh
+prefix:max "%" => id.fv
+prefix:max "#" => id.bv
+
+instance: Subst id id where
+  subst x x' x0 := if x = x0 then x' else x0
+
+def id.splice (i: id) (n δ: ℕ): id :=
+  match i with
+  | %x => if x < n then %x else %(x + δ)
+  | x =>  x
+
+attribute [simp] id.splice.eq_1 id.splice.eq_2
+
+instance bvShift: HAdd id Nat id where
+  hAdd x n := match x with
+  | #x => #(x + n)
+  | _ => x
+
+-- qualifiers
+
+abbrev ql := Finset id
+abbrev qnat := Finset.range
+attribute [sets] Finset.instHasSubset
+attribute [default_instance] Finset.instSingleton
+
+def qdom (fr: Bool) (bvs fvs: Nat): ql :=
+  ?[fr] {✦} ∪ (qnat bvs).image (# ·) ∪ (qnat fvs).image (% ·)
+
+@[sets]
+def closed_ql (fr: Bool) (bvs fvs: Nat) (q: ql): Prop :=
+  q ⊆ qdom fr bvs fvs
+
+def closed_ql.fvs f (q: ql) := ∀⦃x⦄, %x ∈ q → x < f
+
+instance: Subst ql ql where
+  subst x xs q := q \ {x} ∪ ?[x ∈ q] xs
+
+@[simp]
+instance: Subst ql id where
+  subst x x' q := [x ↦ {x'}] q
+
+@[simp]
+instance: Subst ql (id × ql) where
+  subst x xs t := [x ↦ {xs.1} ∪ xs.2] t
+
+def ql.splice (q: ql) (n δ: ℕ): ql :=
+  q.image (id.splice · n δ)
+
+attribute [simp← low] ql.splice.eq_1
+
+instance bvsShift: HAdd ql ℕ ql where
+  hAdd q n := q.image (· + n)
+
+-- type definitions
+
+inductive ty : Type where
+| TTop  : ty
+| TBool  : ty
+| TRef   : ty → ql → ty
+| TFun   : ty → ql → ty → ql → ty
+| TVar   : id → ty
+| TAll   : ty → ql → ty → ql → ty
+deriving DecidableEq
+
+def ty.unfoldable (t: ty) :=
+  match t with
+  | .TTop | .TBool | .TRef _ _ | .TFun _ _ _ _ | .TVar _ | .TAll _ _ _ _ => True
+
+attribute [simp] ty.unfoldable.eq_1 ty.unfoldable.eq_2 ty.unfoldable.eq_3
+attribute [simp] ty.unfoldable.eq_4 ty.unfoldable.eq_5 ty.unfoldable.eq_6
+
+inductive occ_flag where
+| none | no_covariant | no_contravariant | noneq
+deriving DecidableEq
+
+def occ_flag.flip (f: occ_flag): occ_flag :=
+  match f with
+  | .no_covariant => .no_contravariant
+  | .no_contravariant => .no_covariant
+  | _ => f
+
+def occ_flag.tighten (f: occ_flag): occ_flag :=
+  match f with
+  | .noneq => .noneq
+  | _ => .none
+
+attribute [simp] occ_flag.flip.eq_1 occ_flag.flip.eq_2 occ_flag.flip.eq_3
+attribute [simp] occ_flag.tighten.eq_1 occ_flag.tighten.eq_2
+
+def occurs (f: occ_flag) (T: ty) (x: id): Prop :=
+  match T with
+  | .TRef T q =>
+    occurs f.tighten T x ∧ x+1 ∉ q
+  | .TFun T1 q1 T2 q2 =>
+    occurs f.flip T1 (x+1) ∧ (f = .no_covariant ∨ x+1 ∉ q1) ∧
+    occurs f T2 (x+2) ∧ (f = .no_contravariant ∨ x+2 ∉ q2)
+  | .TVar a =>
+    f = .noneq ∨ x ≠ a
+  | .TAll T1 q1 T2 q2 =>
+    occurs f.flip T1 (x+1) ∧ (f = .no_covariant ∨ x+1 ∉ q1) ∧
+    occurs f T2 (x+2) ∧ (f = .no_contravariant ∨ x+2 ∉ q2)
+  | .TTop | .TBool => True
+
+def closed_ty (bv fv: Nat): ty → Prop
+  | .TTop | .TBool => True
+  | .TRef T q =>
+    closed_ty bv fv T ∧
+    closed_ql false (bv+1) fv q
+  | .TFun T1 q1 T2 q2 =>
+    closed_ty (bv+1) fv T1 ∧
+    closed_ty (bv+2) fv T2 ∧
+    closed_ql true (bv+1) fv q1 ∧
+    closed_ql true (bv+2) fv q2 ∧
+    (#0 ∈ q1 → ✦ ∈ q1) ∧
+    occurs .no_covariant T1 #0 ∧
+    occurs .no_contravariant T2 #0
+  | .TVar x => x ∈ qdom false bv fv
+  | .TAll T1 q1 T2 q2 =>
+    closed_ty (bv+1) fv T1 ∧
+    closed_ty (bv+2) fv T2 ∧
+    closed_ql true (bv+1) fv q1 ∧
+    closed_ql true (bv+2) fv q2 ∧
+    (#0 ∈ q1 → ✦ ∈ q1) ∧
+    occurs .no_covariant T1 #0 ∧
+    occurs .no_contravariant T2 #0
+
+@[simp]
+def ty.open (x x': id) (t: ty): ty :=
+  match t with
+  | .TRef T q => .TRef (ty.open x x' T) ([x+1 ↦ x'+1] q)
+  | .TFun T1 q1 T2 q2 =>
+    .TFun (ty.open (x+1) (x'+1) T1) ([x+1 ↦ x'+1] q1)
+          (ty.open (x+2) (x'+2) T2) ([x+2 ↦ x'+2] q2)
+  | .TVar x0 => .TVar ([x ↦ x'] x0)
+  | .TAll T1 q1 T2 q2 =>
+    .TAll (ty.open (x+1) (x'+1) T1) ([x+1 ↦ x'+1] q1)
+          (ty.open (x+2) (x'+2) T2) ([x+2 ↦ x'+2] q2)
+  | .TTop | .TBool => t
+
+instance: Subst ty id where
+  subst := ty.open
+
+@[simp low]
+lemma ty.open_fold {t: ty} {x x': id}:
+  t.open x x' = [x ↦ x'] t :=
+by
+  simp only [subst]
+
+@[simp]
+def ty.open_unfold {t: ty} {x x'} (_: t.unfoldable) :=
+  Eq.symm (@ty.open_fold t x x')
+
+@[simp]
+def ty.TFun' (n: ℕ) T1 q1 T2 q2 :=
+  ty.TFun T1 q1 ([%(n+1) ↦ #1] [%n ↦ #0] T2) ([%(n+1) ↦ #1] [%n ↦ #0] q2)
+
+@[simp]
+def ty.TAll' (n: ℕ) T1 q1 T2 q2 :=
+  ty.TAll T1 q1 ([%(n+1) ↦ #1] [%n ↦ #0] T2) ([%(n+1) ↦ #1] [%n ↦ #0] q2)
+
+@[simp]
+def ty.subst' (x: id) (xt: ty) (xs: ql) (t: ty): ty :=
+  match t with
+  | .TRef T q => .TRef (ty.subst' x xt xs T) ([x+1 ↦ xs] q)
+  | .TFun T1 q1 T2 q2 =>
+    .TFun (ty.subst' (x+1) xt xs T1) ([x+1 ↦ xs] q1)
+          (ty.subst' (x+2) xt xs T2) ([x+2 ↦ xs] q2)
+  | .TAll T1 q1 T2 q2 =>
+    .TAll (ty.subst' (x+1) xt xs T1) ([x+1 ↦ xs] q1)
+          (ty.subst' (x+2) xt xs T2) ([x+2 ↦ xs] q2)
+  | .TVar a => if x = a then xt else .TVar a
+  | .TTop | .TBool => t
+
+instance: Subst ty (ty × ql) where
+  subst x x' t := ty.subst' x x'.1 x'.2 t
+
+@[simp low]
+lemma ty.subst_fold: ty.subst' x xt xs t = [x ↦ (xt, xs)] t := by
+  simp only [instSubstTyProdQl]
+
+@[simp]
+def ty.subst_unfold {x t' q'} {t: ty} (_: t.unfoldable) :=
+  Eq.symm (@ty.subst_fold x t' q' t)
+
+@[simp]
+instance: Subst ty ql where
+  subst x xs t := [x ↦ (ty.TTop, xs)] t
+
+@[simp]
+instance: Subst ty (id × ql) where
+  subst x xs t := [x ↦ (ty.TVar xs.1, {xs.1} ∪ xs.2)] t
+
+def ty.splice (t: ty) (n δ: ℕ): ty :=
+  match t with
+  | .TRef T q => .TRef (T.splice n δ) (q.splice n δ)
+  | .TFun T1 q1 T2 q2 =>
+    .TFun (T1.splice n δ) (q1.splice n δ) (T2.splice n δ) (q2.splice n δ)
+  | .TVar x => .TVar (x.splice n δ)
+  | .TAll T1 q1 T2 q2 =>
+    .TAll (T1.splice n δ) (q1.splice n δ) (T2.splice n δ) (q2.splice n δ)
+  | _ => t
+
+-- typing environment
+
+inductive binding where | var | self | tvar
+deriving DecidableEq
+
+abbrev tenv := List (ty × ql × binding)
+
+def telescope (env: tenv) := forall ⦃x T q1 bn⦄,
+  env[x]? = some (T, q1, bn) → closed_ty 0 x T ∧ closed_ql true 0 x q1
+
+def vars_trans (env: tenv): ql /- q -/ → ql :=
+  -- match env with
+  env.reverseRecOn
+  -- | [] => q
+    (fun q => q)
+  -- | env ++ [(_, q')] => vars_trans env q ∪ ?[...] vars_trans env q'
+    (fun x (_, q', _) f q => f (q ∪ ?[%‖x‖ ∈ q] q'))
+
+abbrev gfset := Finset ℕ  -- growable selfrefs
+
+def ctx_grow (G G': tenv) (growables: gfset): Prop :=
+  ‖G‖ = ‖G'‖ ∧ (∀ i, G[i]? = G'[i]? ∨
+    i ∈ growables ∧ ∃ T q q', q ⊆ q' ∧ closed_ql (✦ ∈ q) 0 i q' ∧
+      G[i]? = some (T, q, .self) ∧ G'[i]? = some (T, q', .self))
+
+-- term language
+
+inductive tm: Type where
+| ttrue
+| tfalse
+| tvar (x: ℕ)
+| tref (t: tm)
+| tget (t: tm)
+| tput (tr tx: tm)
+| tapp (tf tx: tm)
+| tabs (t: tm)
+| tabsa (T: ty) (q: ql) (t: tm)
+| ttapp (tf: tm) (T: ty) (q: ql)
+| ttabs (T: ty) (q: ql) (t: tm)
+| tanno (t: tm) (T: ty) (q: ql)
+
+@[match_pattern] def tm.tlet t1 t2 := (tm.tabs t2).tapp t1
+@[match_pattern] def tm.tlet' t1 T q t2 := tm.tlet (tm.tanno t1 T q) t2
+
+-- semantics
+
+inductive vl: Type where
+| vbool (b: Bool)
+| vref (l: Nat)
+| vabs (H: List vl) (t: tm)
+| vtabs (H: List vl) (t: tm)
+
+abbrev venv := List vl
+abbrev stor := List vl
+
+def teval (n: Nat) (M: stor) (env: venv) (t: tm): Except String (Nat × stor × vl) := do
+  match n, t with
+  | 0, _ => throw "timeout"
+  | _ + 1, .ttrue => return (1, M, .vbool true)
+  | _ + 1, .tfalse => return (1, M, .vbool false)
+  | _ + 1, .tvar x =>
+    match env[x]? with
+    | some v => return (1, M, v)
+    | _ => throw "error"
+  | n + 1, .tref ex =>
+    let (dx, M', vx) ← teval n M env ex
+    return (1+dx, M'++[vx], .vref ‖M'‖)
+  | n + 1, .tget ex =>
+    let (dx, M', vx) ← teval n M env ex
+    match vx with
+    | .vref x =>
+      match M'[x]? with
+      | some v => return (1+dx, M', v)
+      | _ => throw "error"
+    | _ => throw "error"
+  | n + 1, .tput er ex =>
+    let (dr, M', vr) ← teval n M env er
+    match vr with
+    | .vref x =>
+      let (dx, M'', vx) ← teval n M' env ex
+      match M''[x]? with
+      | some _ => return (1+dr+dx, M''.set x vx, .vbool true)
+      | _ => throw "error"
+    | _ => throw "error"
+  | _ + 1, .tabs y => return (1, M, .vabs env y)
+  | _ + 1, .tabsa _ _ y => return (1, M, .vabs env y)
+  | n + 1, .tapp ef ex =>
+    let (df, M', vf) ← teval n M env ef
+    match vf with
+    | .vabs env2 ey =>
+      let (dx, M'', vx) ← teval n M' env ex
+      let (dy, M''', ry) ← teval n M'' (env2 ++ [.vabs env2 ey, vx]) ey
+      return (1+df+dx+dy, M''', ry)
+    | _ => throw "error"
+  | _ + 1, .ttabs _ _ y => return (1, M, .vtabs env y)
+  | n + 1, .ttapp ef _ _ =>
+    let (df, M', vf) ← teval n M env ef
+    match vf with
+    | vf@(.vtabs env2 ey) =>
+      let (dy, M'', ry) ← teval n M' (env2 ++ [vf, .vbool false]) ey
+      return (1+df+dy, M'', ry)
+    | _ => throw "error"
+  | n + 1, .tanno t _ _ =>
+    let (d, M', vf) ← teval n M env t
+    return (1+d, M', vf)
