checking/coq_v1/README.md
@@ -1,0 +1,68 @@
+# Expressive Reachability Types with Sound and Decidable Bidirectional Type Checking
+
+## Overview
+
+* `lambda_diamond_R.v`:
+    Bidirectional type system $\lambda^\diamond_R$ with decidable type checking/inference, including refined subtyping for self-references [2].
+* `lambda_diamond_E.v`:
+    Type system $\lambda^\diamond_E$.
+
+## Mechanization Outline ([`lambda_diamond_R.v`](lambda_diamond_R.v))
+
+| Section | Item | Mechanization | Paper |
+|---------|------|---------------|-------|
+| Syntactic Definitions | Term Typing   | `Inductive has_type` | $\S 3.2$ |
+|                       | Subtyping     | `Inductive stp`      | $\S 3.3$ |
+|                       | Subqualifying | `Inductive qstp`     | $\S 3.3$ |
+| Semantic Definitions | Bigstep Interpreter    | `Fixpoint teval`      |
+|                      | Value Interpretation   | `Fixpoint val_type`   |
+|                      | Semantic Typing        | `Definition sem_type` |
+|                      | Semantic Subtyping     | `Definition sem_stp2` |
+|                      | Semantic Subqualifying | `Definition sem_qstp` |
+|                      | various semantic typing rules | ... |
+| Metatheory | Subqualifying | `Theorem qstp_fundamental`  |
+|            | Subtyping     | `Theorem stp2_fundamental`  |
+|            | Typing        | `Theorem full_total_safety` | $\S 3.4$ |
+| Typing Examples | Box (v1) | Transparent `Lemma t_box_transparent`,<br>`Lemma t_unbox_transparent`,<br>`Lemma ex_box_unbox_transparent1` |
+|                 |          | Opaque `Lemma t_unbox_opaque1` |
+|                 | Box (v2) | Transparent `Lemma t_box_transparent2`,<br>`Lemma t_unbox_transparent2`,<br>`Lemma ex_box_unbox_transparent2` |
+|                 |          | Opaque `Lemma t_unbox_opaque2` |
+|                 |          | Subtyping `Lemma upcast_box`, `Lemma ex_escape1` |
+|                 | Pair     | Transparent `Lemma t_pair_transparent`,<br>`Lemma t_fst_transparent`,<br>`Lemma t_snd_transparent` |
+|                 |          | Opaque `Lemma TPair_opaque_fst`,<br>`Lemma TPair_opaque_snd` |
+|                 |          | Subtyping `Lemma t_pair_trans_to_opaque` |
+| Typing Algorithm | Qualifier Upcast     | `Definition get_qstp`,<br>`Lemma get_qstp_is_sound`         | $\S 4.1$ |
+|                  | Qualifier Checking   | `Definition check_qstp`,<br>`Lemma check_qstp_is_sound`     | $\S 4.1$ |
+|                  | Subtype Checking     | `Fixpoint upcast`,<br>`Lemma upcast_is_sound`               | $\S 4.2$ |
+|                  | Avoidance Algorithm  | `Fixpoint avoidance`,<br>`Lemma avoidance_is_sound`         | $\S 4.3$ |
+|                  | Bidirectional Typing | `Fixpoint bidirectional`,<br>`Lemma bidirectional_is_sound` | $\S 4.4$ |
+| Type Checking Examples | Subtype Checking    | `Example upcast_with_pair`          |
+|                        | Avoidance Algorithm | `Example avoidance_with_pair_{a,b}` |
+|                        | End-to-End Example  | `Definition pair_example`           | $\S 5$ |
+
+The typing and subtyping of $\lambda^\diamond_E$ shares same names as $\lambda^\diamond_R$ mechanization. Examples and algorithms are not included in the mechanization of $\lambda^\diamond_E$.
+
+## References
+
+[1] **Modeling Reachability Types with Logical Relations: Semantic Type Soundness, Termination, and Equational Theory** (arXiv 2023)</br>
+Yuyan Bao, Guannan Wei, Oliver Bračevac, Tiark Rompf
+([pdf](https://arxiv.org/pdf/2309.05885.pdf)).
+
+[2] **Escape with Your Self: Expressive Reachability Types with Sound and Decidable Bidirectional Type Checking** </br>
+Songlin Jia, Guannan Wei, Siyuan He, Yueyang Tang, Yuyan Bao, Tiark Rompf
+([pdf](https://arxiv.org/pdf/2404.08217.pdf)).
+
+
+## Compilation
+
+To generate/update the `CoqMakefile` from `_CoqProject`:
+
+`coq_makefile -f _CoqProject -o CoqMakefile`
+
+Then, to compile/check all proof scripts listed in `_CoqProject`:
+
+`make -f CoqMakefile all`
+
+Compatibility tested with Coq `8.17.1`.
+
+
